src/RqRsInvMsg.v
@@ -1,0 +1,255 @@
+Require Import Peano_dec Omega List ListSupport.
+Require Import Common FMap.
+Require Import Syntax Semantics SemFacts StepM Invariant Serial.
+Require Import Reduction Commutativity QuasiSeq Topology.
+Require Import RqRsTopo RqRsFacts.
+
+Set Implicit Arguments.
+
+Open Scope list.
+Open Scope fmap.
+
+Section FootprintInv.
+  Context {oifc: OStateIfc}.
+  Variables (dtr: DTree)
+            (sys: System oifc).
+
+  Hypothesis (Hitr: GoodRqRsSys dtr sys).
+
+  Definition FootprintUpOkEx (oidx: IdxT) (rqi: RqInfo Msg) :=
+    exists rqFrom rqTo rsFrom rsbTo,
+      rqi.(rqi_minds_rss) = [rsFrom] /\
+      rqi.(rqi_midx_rsb) = rsbTo /\
+      FootprintUpOk dtr oidx rqFrom rqTo rsFrom rsbTo.
+
+  Definition FootprintDownOkEx (oidx: IdxT) (rqi: RqInfo Msg) :=
+    exists rqFrom rqTos rssFrom rsbTo,
+      rqi.(rqi_minds_rss) = rssFrom /\
+      rqi.(rqi_midx_rsb) = rsbTo /\
+      (FootprintUpDownOk dtr oidx rqFrom rqTos rssFrom rsbTo \/
+       FootprintDownDownOk dtr oidx rqFrom rqTos rssFrom rsbTo).
+
+  Definition FootprintsOkORqs (orqs: ORqs Msg) :=
+    forall oidx,
+      orqs@[oidx] >>=[True]
+          (fun orq =>
+             (orq@[upRq] >>=[True] (fun rqiu => FootprintUpOkEx oidx rqiu)) /\
+             (orq@[downRq] >>=[True] (fun rqid => FootprintDownOkEx oidx rqid))).
+
+  Lemma footprints_ok_orqs_add:
+    forall orqs,
+      FootprintsOkORqs orqs ->
+      forall oidx norq,
+        norq@[upRq] >>=[True] (fun rqiu => FootprintUpOkEx oidx rqiu) ->
+        norq@[downRq] >>=[True] (fun rqid => FootprintDownOkEx oidx rqid) ->
+        FootprintsOkORqs (orqs +[oidx <- norq]).
+  Proof.
+    unfold FootprintsOkORqs; intros.
+    mred; simpl; intros; auto.
+  Qed.
+  
+  Definition FootprintsOk (st: MState oifc) :=
+    FootprintsOkORqs st.(bst_orqs).
+
+  Ltac disc_rule_custom ::=
+    repeat
+      match goal with
+      | [H1: FootprintsOkORqs ?orqs, H2: ?orqs @[?oidx] = _ |- _] =>
+        let Hf := fresh "H" in
+        pose proof (H1 oidx) as Hf;
+        rewrite H2 in Hf; simpl in Hf; dest;
+        clear H2
+      end.
+
+  Lemma footprints_ok_init:
+    InvInit sys FootprintsOk.
+  Proof.
+    intros; do 3 red.
+    intros; simpl; auto.
+  Qed.
+  
+  Lemma footprints_ok_step:
+    InvStep sys step_m FootprintsOk.
+  Proof.
+    red; intros.
+    red in H0; red.
+    inv H1; try assumption.
+
+    simpl in *.
+    good_rqrs_rule_get rule.
+    good_rqrs_rule_cases rule.
+
+    - disc_rule_conds.
+      mred.
+      apply footprints_ok_orqs_add; auto; try (mred; fail).
+    - disc_rule_conds.
+      mred.
+      apply footprints_ok_orqs_add; auto; try (mred; fail).
+    - disc_rule_conds.
+      + apply footprints_ok_orqs_add; disc_rule_conds; auto.
+        * do 4 eexists; repeat split; eassumption.
+        * rewrite <-H20; assumption.
+      + apply footprints_ok_orqs_add; disc_rule_conds; auto.
+        * rewrite <-H19; assumption.
+        * do 4 eexists; repeat split.
+          left; eassumption.
+      + apply footprints_ok_orqs_add; disc_rule_conds; auto.
+        * rewrite <-H19; assumption.
+        * do 4 eexists; repeat split.
+          right; eassumption.
+    - disc_rule_conds.
+      + apply footprints_ok_orqs_add; disc_rule_conds; auto.
+        rewrite <-H15; assumption.
+      + apply footprints_ok_orqs_add; disc_rule_conds; auto.
+        rewrite <-H15; assumption.
+    - disc_rule_conds.
+      apply footprints_ok_orqs_add; disc_rule_conds; auto.
+      do 4 eexists; repeat split.
+      left; eassumption.
+  Qed.
+
+  Lemma footprints_ok:
+    InvReachable sys step_m FootprintsOk.
+  Proof.
+    eapply inv_reachable.
+    - apply footprints_ok_init.
+    - apply footprints_ok_step.
+  Qed.
+  
+End FootprintInv.
+
+Ltac good_footprint_get oidx :=
+  match goal with
+  | [Hfpok: FootprintsOk _ _, Ho: _@[oidx] = Some _ |- _] =>
+    let H := fresh "H" in
+    pose proof Hfpok as H;
+    specialize (H oidx); simpl in H
+  end.
+
+Ltac disc_footprints_ok :=
+  repeat
+    match goal with
+    | [H: FootprintsOk _ _ |- _] => red in H
+    | [H1: FootprintsOkORqs _ ?orqs, H2: ?orqs @[?oidx] = _ |- _] =>
+      let Hf := fresh "H" in
+      pose proof (H1 oidx) as Hf;
+      rewrite H2 in Hf; simpl in Hf; dest;
+      clear H2
+    | [H: FootprintUpOkEx _ _ _ |- _] =>
+      let rqFrom := fresh "rqFrom" in
+      let rqTo := fresh "rqTo" in
+      let rsFrom := fresh "rsFrom" in
+      let rsbTo := fresh "rsbTo" in
+      destruct H as [rqFrom [rqTo [rsFrom [rsbTo ?]]]]; dest
+    | [H: FootprintDownOkEx _ _ _ |- _] =>
+      let rqFrom := fresh "rqFrom" in
+      let rqTos := fresh "rqTos" in
+      let rssFrom := fresh "rssFrom" in
+      let rsbTo := fresh "rsbTo" in
+      destruct H as [rqFrom [rqTos [rssFrom [rsbTo ?]]]]; dest
+                                                   
+    | [H: FootprintUpOk _ _ _ _ _ _ |- _] =>
+      let cidx := fresh "cidx" in
+      destruct H as [cidx ?]; dest
+    | [H: FootprintUpDownOk _ _ _ _ _ _ \/
+          FootprintDownDownOk _ _ _ _ _ _ |- _] => destruct H
+    | [H: exists _, FootprintUpDownOk _ _ _ _ _ _ |- _] =>
+      let rsFrom := fresh "rqFrom" in
+      destruct H as [rqFrom ?]; dest
+    | [H: FootprintUpDownOk _ _ _ _ _ _ |- _] =>
+      let upCIdx := fresh "upCIdx" in
+      destruct H as [upCIdx ?]; dest
+    | [H: FootprintDownDownOk _ _ _ _ _ _ |- _] => red in H; dest
+    end.
+
+Section MessageInv.
+  Context {oifc: OStateIfc}.
+  Variables (dtr: DTree)
+            (sys: System oifc).
+
+  Hypothesis (Hitr: GoodRqRsSys dtr sys).
+
+  Definition RqUpMsgs (oidx: IdxT) (msgs: list (Id Msg)): Prop :=
+    exists cidx rqUp,
+      msgs = [rqUp] /\
+      msg_type (valOf rqUp) = MRq /\
+      parentIdxOf dtr cidx = Some oidx /\
+      rqEdgeUpFrom dtr cidx = Some (idOf rqUp).
+
+  Definition RqDownMsgs (oidx: IdxT) (msgs: list (Id Msg)): Prop :=
+    exists rqDown, msgs = [rqDown] /\
+                   msg_type (valOf rqDown) = MRq /\
+                   edgeDownTo dtr oidx = Some (idOf rqDown).
+
+  Definition RsUpMsgs (oidx: IdxT) (msgs: list (Id Msg)): Prop :=
+    Forall (fun msg => msg_type (valOf msg) = MRs) msgs /\
+    Forall (fun rs => exists cidx, rsEdgeUpFrom dtr cidx = Some rs)
+           (idsOf msgs).
+
+  Definition RsDownMsgs (oidx: IdxT) (msgs: list (Id Msg)): Prop :=
+    exists rsDown, msgs = [rsDown] /\
+                   msg_type (valOf rsDown) = MRs /\
+                   edgeDownTo dtr oidx = Some (idOf rsDown).
+  
+  Ltac disc_rule_custom ::=
+    disc_footprints_ok.
+  
+  Lemma messages_in_cases:
+    forall st1 oidx ridx rins routs st2,
+      Reachable (steps step_m) sys st1 ->
+      step_m sys st1 (RlblInt oidx ridx rins routs) st2 ->
+      RqUpMsgs oidx rins \/
+      RqDownMsgs oidx rins \/
+      RsUpMsgs oidx rins \/
+      RsDownMsgs oidx rins.
+  Proof.
+    intros.
+
+    (* Register some necessary invariants to prove this invariant. *)
+    pose proof (footprints_ok Hitr H).
+
+    inv H0.
+    good_rqrs_rule_get rule.
+    good_rqrs_rule_cases rule.
+
+    - left.
+      disc_rule_conds.
+      solve_rule_conds.
+
+    - right; left.
+      disc_rule_conds.
+      solve_rule_conds.
+
+    - disc_rule_conds.
+      + left; solve_rule_conds.
+      + left; solve_rule_conds.
+      + right; left; solve_rule_conds.
+
+    - disc_rule_conds.
+      + right; right; right.
+        rewrite H4 in H2.
+        disc_rule_conds.
+        solve_rule_conds.
+      + right; right; left.
+        rewrite H2 in H23.
+        split; auto.
+        clear -H23; apply Forall_forall; intros.
+        eapply RqRsDownMatch_rs_In in H23; [|eassumption].
+        dest; eauto.
+      + right; right; left.
+        rewrite H2 in H22.
+        split; auto.
+        clear -H22; apply Forall_forall; intros.
+        eapply RqRsDownMatch_rs_In in H22; [|eassumption].
+        dest; eauto.
+
+    - right; right; right.
+      disc_rule_conds.
+      solve_rule_conds.
+  Qed.
+    
+End MessageInv.
+
+Close Scope list.
+Close Scope fmap.
+
